Add [_auto_unchanged_node_vals_stays_valid0] for original nodes unchanged

ind/DoublyLinkedListIface.fst
@@ -318,6 +318,26 @@ let _auto_unchanged_node_vals_stays_valid h0 h1 d d2 =
     | n :: ns -> aux ns in
   aux (as_list h1 d)
 
+(** If a dll is assigned to, its original nodes stay unchanged *)
+val _auto_unchanged_node_vals_stays_valid0 (h0 h1:HS.mem) (d:dll 'a) :
+  Lemma
+    (requires (B.modifies (B.loc_buffer d) h0 h1 /\
+               B.loc_buffer d `B.loc_disjoint` DLL.dll_fp0 (d@h0) /\
+               B.live h0 d))
+    (ensures (unchanged_node_vals h0 h1 (as_list h0 d)))
+    [SMTPat (B.modifies (B.loc_buffer d) h0 h1);
+     SMTPat (unchanged_node_vals h0 h1 (as_list h0 d))]
+let _auto_unchanged_node_vals_stays_valid0 h0 h1 d =
+  let rec aux nl : Lemma
+    (requires (
+       B.modifies (B.loc_buffer d) h0 h1 /\
+       DLL.nodelist_fp0 nl `B.loc_disjoint` B.loc_buffer d))
+    (ensures (unchanged_node_vals h0 h1 nl)) =
+    match nl with
+    | [] -> ()
+    | n :: ns -> aux ns in
+  aux (as_list h0 d)
+
 (** If a node belongs to a dll, then its fp is included *)
 let rec _lemma_node_in_list_is_included (n:node 'a) (nl:list (node 'a)) :
   Lemma
